Finished upper bond proofs

specs/Spec.Package.Merge.fst
@@ -9,35 +9,449 @@ let rec lemma_weight_sorted w i j =
   | _ -> if length w > 2 then lemma_weight_sorted (tail w) (i - 1) (j - 1)
 #pop-options
 
-#push-options "--fuel 1 --ifuel 1 --z3rlimit 128"
-let rec lemma_row_weight_sorted #w #e #c #p s i j =
+#push-options "--fuel 2 --ifuel 1 --z3rlimit 128"
+let rec lemma_row_weight_sorted
+  #w #e #c #p (s:row_t w e c p{row_sorted s}) (i j: nat): Lemma
+  (requires i < j /\ i < c + p /\ j < c + p)
+  (ensures s.(i) `lt` s.(j))
+  (decreases %[c + p; j - i]) =
   if j = c + p - 1 then begin
     if j - i > 1 then lemma_row_weight_sorted s i (j - 1)
   end else
     lemma_row_weight_sorted (unsnoc s) i j
 
-let rec lemma_last_item_gte_last_leaf #w #e #c #p (s: row w e c p): Lemma
-  (requires c >= 1)
+let rec lemma_last_item_gte_last_coin #w #e #c #p (s: row_t w e c p): Lemma
+  (requires c >= 1 /\ row_sorted s)
   (ensures weight s.(c + p - 1) >= w.[c - 1]) =
   match s with
   | SHead _ | SCoin _ _ -> ()
-  | SPackage xs x -> lemma_last_item_gte_last_leaf xs
+  | SPackage xs x -> lemma_last_item_gte_last_coin xs
+#pop-options
 
-#push-options "--fuel 1 --ifuel 0 --z3rlimit 1024 --z3refresh --query_stats"
-let lemma_pkg_weight #w #n #e #p #c' #p' prev s =
+#push-options "--fuel 2 --ifuel 0 --z3rlimit 1024 --query_stats"
+let lemma_pkg_weight_sorted #w (#e: pos)
+  #p (prev: row w (e + 1) (length w) p)
+  #c' #p' (s: row w e c' p'): Lemma
+  (requires
+    merge_element_lt prev s /\
+    (pkg_smaller prev s \/ coin_smaller prev s))
+  (ensures
+    (pkg_smaller prev s ==>
+      row_sorted (SPackage s (Package prev.(p' * 2) prev.(p' * 2 + 1)))) /\
+    (coin_smaller prev s ==> row_sorted (SCoin s (Coin e w.[c'])))) = ()
+
+let lemma_pkg_weight_unpack #w (#e: pos)
+  #p (prev: row w (e + 1) (length w) p)
+  #c' #p' (s: row w e c' p'{unpack_correspond prev s}): Lemma
+  (requires
+    merge_element_lt prev s /\
+    (pkg_smaller prev s \/ coin_smaller prev s))
+  (ensures
+    (pkg_smaller prev s ==>
+      unpack_correspond prev (SPackage s (Package prev.(p' * 2) prev.(p' * 2 + 1)))) /\
+    (coin_smaller prev s ==> unpack_correspond prev (SCoin s (Coin e w.[c'])))) = ()
+#pop-options
+
+#push-options "--fuel 1 --ifuel 1 --z3rlimit 1024 --query_stats"
+let rec lemma_row_first #w #e #c #p (s: row_t w e c p): Lemma
+  (ensures
+    row_item_weight s 0 == w.[0] /\
+    s.(0) == Coin e w.[0] /\
+    weight s.(0) == weight (prefix s 1)) =
+  match s with
+  | SHead _ -> ()
+  | SCoin xs _ -> lemma_row_first xs
+  | SPackage xs _ -> lemma_row_first xs
+
+#push-options "--fuel 2 --ifuel 1 --z3rlimit 1024 --query_stats"
+let rec lemma_prefix_cnt_inv #w #e #c #p (s: row_t w e c p) (i: pos{i <= c + p}): Lemma
+  (ensures prefix_coin_cnt s i + prefix_pkg_cnt s i == i) =
+  if i < c + p then
+    match s with | SCoin xs _ | SPackage xs _ -> lemma_prefix_cnt_inv xs i
+
+let rec lemma_eq_elim #w #e #c #p (a: row_t w e c p) #c' #p' (b: row_t w e c' p'): Lemma
+  (requires c == c' /\ p == p' /\
+    (forall i. row_item_weight a i == row_item_weight b i /\ a.(i) == b.(i)))
+  (ensures a == b) =
+  assert(a.(c + p - 1) == b.(c + p - 1));
+  if c + p > 1 then match a with
+  | SCoin a' _ -> (match b with | SCoin b' _ ->
+    assert(forall i. i < c + p - 1 ==> row_item_weight a i == row_item_weight a' i);
+    assert(forall i. i < c + p - 1 ==> row_item_weight b i == row_item_weight b' i);
+    lemma_eq_elim a' b')
+  | SPackage a' _ -> (match b with | SPackage b' _ ->
+    assert(forall i. i < c + p - 1 ==> row_item_weight a i == row_item_weight a' i);
+    assert(forall i. i < c + p - 1 ==> row_item_weight b i == row_item_weight b' i);
+    lemma_eq_elim a' b')
+
+let rec lemma_prefix_prefix_aux #w #e #c #p (s: row_t w e c p)
+  (i: pos{i <= c + p}) (j: pos{j <= i}): Lemma
+  (ensures (
+    lemma_prefix_cnt_inv s i;
+    prefix_coin_cnt (prefix s i) j == prefix_coin_cnt s j /\
+    prefix_pkg_cnt (prefix s i) j == prefix_pkg_cnt s j)) =
+  lemma_prefix_cnt_inv s i;
+  if j < i && i < c + p then
+    match s with
+    | SCoin s' _ -> lemma_prefix_prefix_aux s' i j
+    | SPackage s' _ -> lemma_prefix_prefix_aux s' i j
+
+let rec lemma_prefix_prefix #w #e #c #p (s: row_t w e c p)
+  (i: pos{i <= c + p}) (j: pos{j <= i}): Lemma
+  (ensures (
+    lemma_prefix_cnt_inv s i;
+    lemma_prefix_prefix_aux s i j;
+    prefix (prefix s i) j == prefix s j)) =
+  lemma_prefix_cnt_inv s i;
+  if j < i && i < c + p then
+    match s with | SCoin s' _ | SPackage s' _ -> lemma_prefix_prefix s' i j
+
+let rec lemma_prefix_eq_aux #w #e #c #p
+  (s: row_t w e c p) (i: pos{i <= c + p}) (j: nat{j < i}): Lemma
+  (ensures (
+    lemma_prefix_cnt_inv s i;
+    row_item_weight (prefix s i) j == row_item_weight s j)) =
+  if j < i && i < c + p then
+    match s with | SCoin s' _ | SPackage s' _ -> lemma_prefix_eq_aux s' i j
+
+let rec lemma_prefix_eq #w #e #c #p
+  (s: row_t w e c p) (i: pos{i <= c + p}) (j: nat{j < i}): Lemma
+  (ensures (
+    lemma_prefix_eq_aux s i j;
+    lemma_prefix_cnt_inv s i;
+    (prefix s i).(j) == s.(j))) =
+  if j < i && i < c + p then
+    match s with | SCoin s' _ | SPackage s' _ -> lemma_prefix_eq s' i j
+  
+let lemma_prefix_weight #w #e #c #p (s: row_t w e c p) (i: pos{i <= c + p}): Lemma
+  (requires i > 1)
+  (ensures weight (prefix s i) = weight (prefix s (i - 1)) + weight s.(i - 1)) =
+  let s' = prefix s i in
+  lemma_prefix_cnt_inv s i;
+  assert(weight s' ==
+    (match s' with
+    | SHead c -> w.[0]
+    | SCoin xs x ->
+      row_weight (prefix s' (i - 1)) + row_item_weight s' (i - 1)
+    | SPackage #_ #_ #_ #_ #wp xs x ->
+      row_weight (prefix s' (i - 1)) + row_item_weight s' (i - 1)));
+  if c + p > 1 then
+    calc (==) {
+      row_weight (prefix s' (i - 1)) + row_item_weight s' (i - 1);
+      =={lemma_prefix_prefix s i (i - 1)}
+      row_weight (prefix s (i - 1)) + row_item_weight s' (i - 1);
+      =={lemma_prefix_eq s i (i - 1)}
+      weight (prefix s (i - 1)) + row_item_weight s (i - 1);
+    }
+#pop-options
+
+#push-options "--fuel 1 --ifuel 0 --z3rlimit 1024 --query_stats"
+let lemma_pkg_weight_equality #w (#e: pos)
+  #p (prev: row w (e + 1) (length w) p)
+  #c' (#p': pkg_cnt c'{p' * 2 <= length w + p})
+  (s: row w e c' p'{row_weight_equality prev s}): Lemma
+  (requires
+    merge_element_lt prev s /\
+    (pkg_smaller prev s \/ coin_smaller prev s))
+  (ensures
+    (pkg_smaller prev s ==>
+      row_weight_equality prev (SPackage s (Package prev.(p' * 2) prev.(p' * 2 + 1)))) /\
+    (coin_smaller prev s ==> row_weight_equality prev (SCoin s (Coin e w.[c'])))) =
+  let n = length w in
+  let pmax = Math.Lib.min (n - 2) ((n + p) / 2) in
+  if p' < pmax then
+    let pkg: item e _ = Package prev.(p' * 2) prev.(p' * 2 + 1) in
+    let s' = SPackage s pkg in
+    if c' = n || weight (Coin e w.[c']) > weight pkg then begin
+      calc (==) {
+        weight (s' <: row_t w e c' (p' + 1));
+        =={}
+        weight (s <: row_t w e c' p') +
+        weight (Package prev.(p' * 2) prev.(p' * 2 + 1));
+      };
+      if p' = 0 then
+        calc (==) {
+          weight (s <: row_t w e c' p') +
+          weight (Package prev.(p' * 2) prev.(p' * 2 + 1));
+          =={}
+          weight_sum (slice w 0 c') +
+          weight prev.(0) + weight prev.(1);
+          =={lemma_row_first prev}
+          weight_sum (slice w 0 c') +
+          weight (prefix prev 1) + weight prev.(1);
+          =={lemma_prefix_weight prev 2}
+          weight_sum (slice w 0 c') + weight (prefix prev 2);
+        }
+      else
+        calc (==) {
+          weight (s <: row_t w e c' p') +
+          weight (Package prev.(p' * 2) prev.(p' * 2 + 1));
+          =={}
+          weight_sum (slice w 0 c') +
+          weight (prefix prev (p' * 2)) + weight prev.(p' * 2) +
+          weight prev.(p' * 2 + 1);
+          =={lemma_prefix_weight prev (p' * 2 + 1)}
+          weight_sum (slice w 0 c') +
+          weight (prefix prev ((p' * 2) + 1)) + weight prev.(p' * 2 + 1);
+          =={lemma_prefix_weight prev (p' * 2 + 2)}
+          weight_sum (slice w 0 c') + weight (prefix prev ((p' * 2) + 2));
+        }
+    end
+
+#push-options "--fuel 2 --ifuel 1"
+let rec lemma_unpack_correspond #w (#e: pos{e > 1}) #c #p 
+  (prev: row_t w e c p) #c' #p' (s: row_t w (e - 1) c' p'): Lemma
+  (requires
+    row_sorted prev /\ row_sorted s /\
+    unpack_correspond prev s /\
+    p' > 0 /\ 2 * p' <= c + p)
+  (ensures
+    weight s.(c' + p' - 1) >=
+    weight (prev.(2 * (p' - 1))) + weight (prev.(2 * (p' - 1) + 1)))
+  (decreases c') =
+  match s with
+  | SCoin xs _ -> lemma_unpack_correspond prev #(c' - 1) #p' xs
+  | SPackage xs x -> ()
+
+let rec lemma_prefix_row_sorted #w #e #c #p (s: row_t w e c p) (i: pos{i <= c + p}): Lemma
+  (requires row_sorted s)
+  (ensures row_sorted (prefix s i)) =
+  if i < c + p then
+    match s with | SCoin xs _ | SPackage xs _ -> lemma_prefix_row_sorted xs i
+
+let lemma_row_monotonous #w (#e: pos{e > 1}) #p 
+  (prev: row w e (length w) p) #c' #p' (s: row w (e - 1) c' p'): Lemma
+  (requires
+    p' > 0 /\ 2 * p' <= length w + p /\
+    unpack_correspond prev s /\
+    merge_element_lt prev s)
+  (ensures prefix_coin_cnt prev (p' * 2) <= c') =
+  if prefix_coin_cnt prev (p' * 2) > c' && c' < length w then begin
+    lemma_prefix_cnt_inv prev (p' * 2);
+    lemma_unpack_correspond prev s;
+    lemma_prefix_row_sorted prev (p' * 2);
+    lemma_prefix_eq prev (p' * 2) (p' * 2 - 1);
+    lemma_last_item_gte_last_coin (prefix prev (p' * 2))
+  end
+
+let rec lemma_weight_monotonous (w: seq pos{length w >= 1}) (i j: pos): Lemma
+  (requires i <= j /\ i <= length w /\ j <= length w)
+  (ensures weight_sum (slice w 0 i) <= weight_sum (slice w 0 j)) =
+  if i < j then lemma_weight_monotonous w i (j - 1)
+#pop-options
+
+#push-options "--fuel 1 --ifuel 0"
+let lemma_pkg_weight_merge_inv #w (#e: pos) (max: pos{max > e})
+  #p (prev: row w (e + 1) (length w) p{row_weight_upper_bound max prev})
+  #c' (#p': pkg_cnt c'{p' * 2 <= length w + p})
+  (s: row w e c' p'{row_weight_equality prev s /\ row_weight_upper_bound max s}): Lemma
+  (requires
+    merge_element_lt prev s /\
+    unpack_correspond prev s /\
+    (pkg_smaller prev s \/ coin_smaller prev s))
+  (ensures (pkg_smaller prev s ==> 
+      merge_element_lt prev (SPackage s (Package prev.(p' * 2) prev.(p' * 2 + 1)))) /\
+    (coin_smaller prev s ==> merge_element_lt prev (SCoin s (Coin e w.[c'])))) =
+  let n = length w in
+  let pmax = Math.Lib.min (n - 2) ((n + p) / 2) in
+  if c' < n && (p' = pmax || weight prev.(p' * 2) + weight prev.(p' * 2 + 1) >= w.[c'])
+  then begin
+    let s' = SCoin s (Coin e w.[c']) in
+    assert(weight s'.(c' + p') == w.[c']);
+    if c' + 1 < n then
+      assert(weight s'.(c' + p') <= w.[c' + 1]);
+    if p' * 2 + 1 < length w + p then
+      assert(weight s'.(c' + p') <= weight prev.(2 * p') + weight prev.(2 * p' + 1))
+  end else if 2 * p' + 3 < n + p then begin
+    lemma_row_weight_sorted prev (p' * 2) (p' * 2 + 1);
+    lemma_row_weight_sorted prev (p' * 2 + 1) (p' * 2 + 2);
+    lemma_row_weight_sorted prev (p' * 2 + 2) (p' * 2 + 3)
+  end
+
+let lemma_pkg_weight_upper_bound_coin_aux #w (#e: pos) (max: pos{max > e})
+  #p (prev: row w (e + 1) (length w) p{row_weight_upper_bound max prev})
+  #c' (#p': pkg_cnt c'{p' * 2 <= length w + p})
+  (s: row w e c' p'{row_weight_equality prev s /\ row_weight_upper_bound max s})
+  (i: pos{i <= c' + p' + 1}) : Lemma
+  (requires merge_element_lt prev s /\ unpack_correspond prev s /\ coin_smaller prev s)
+  (ensures (
+    let s' = SCoin s (Coin e w.[c']) in
+    let c'' = prefix_coin_cnt s' i in
+    weight (prefix s' i) <= (max - e + 1) * weight_sum (slice w 0 c''))) =
+  let n = length w in
+  let pmax = Math.Lib.min (n - 2) ((n + p) / 2) in
+  let s' = SCoin s (Coin e w.[c']) in
+  let c'' = prefix_coin_cnt s' i in
+  if i = c' + p' + 1 then begin
+    calc (==) {
+      weight (prefix s' i);
+      =={lemma_prefix_weight s' i}
+      weight (prefix s (c' + p')) + weight s'.(c' + p');
+      =={}
+      weight (s <: row_t w e c' p') + w.[c'];
+    };
+    if p' = 0 then
+      Math.Lemmas.lemma_mult_le_right (weight_sum (slice w 0 c'')) 1 (max - e + 1)
+    else
+      calc (<=) {
+        weight (prefix s' i);
+        <={}
+        weight_sum (slice w 0 c'') + weight (prefix prev (p' * 2));
+        <={}
+        weight_sum (slice w 0 c'') +
+        (max - e) * weight_sum (slice w 0 (prefix_coin_cnt prev (p' * 2)));
+        <={
+          lemma_row_monotonous prev s;
+          lemma_weight_monotonous w (prefix_coin_cnt prev (p' * 2)) c'';
+          Math.Lemmas.lemma_mult_le_left
+            (max - e)
+            (weight_sum (slice w 0 (prefix_coin_cnt prev (p' * 2))))
+            (weight_sum (slice w 0 c''))
+        }
+        weight_sum (slice w 0 c'') + (max - e) * weight_sum (slice w 0 c'');
+        =={Math.Lemmas.distributivity_add_left 1 (max - e) (weight_sum (slice w 0 c''))}
+        (max - e + 1) * weight_sum (slice w 0 c'');
+      }
+  end
+
+let lemma_pkg_weight_upper_bound_pkg_aux #w (#e: pos) (max: pos{max > e})
+  #p (prev: row w (e + 1) (length w) p{row_weight_upper_bound max prev})
+  #c' (#p': pkg_cnt c'{p' * 2 <= length w + p})
+  (s: row w e c' p'{row_weight_equality prev s /\ row_weight_upper_bound max s})
+  (i: pos{i <= c' + p' + 1}) : Lemma
+  (requires merge_element_lt prev s /\ unpack_correspond prev s /\ pkg_smaller prev s)
+  (ensures (
+    let s' = SPackage s (Package prev.(p' * 2) prev.(p' * 2 + 1)) in
+    let c'' = prefix_coin_cnt s' i in
+    weight (prefix s' i) <= (max - e + 1) * weight_sum (slice w 0 c''))) =
+  let n = length w in
+  let pmax = Math.Lib.min (n - 2) ((n + p) / 2) in
+  let s' = SPackage s (Package prev.(p' * 2) prev.(p' * 2 + 1)) in
+  let c'' = prefix_coin_cnt s' i in
+  if i = c' + p' + 1 then begin
+    calc (==) {
+      weight (prefix s' i);
+      =={lemma_prefix_weight s' i}
+      weight (prefix s (c' + p')) + weight s'.(c' + p');
+      =={}
+      weight (s <: row_t w e c' p') + weight prev.(2 * p') + weight prev.(2 * p' + 1);
+    };
+    lemma_last_item_gte_last_coin s;
+    lemma_pkg_weight_merge_inv max prev s;
+    if p' = 0 then
+      calc (<=) {
+        weight (prefix s' i);
+        <={}
+        weight_sum (slice w 0 c'') + weight prev.(0) + weight prev.(1);
+        <={lemma_row_first prev}
+        weight_sum (slice w 0 c'') + weight (prefix prev 1) + weight prev.(1);
+        <={lemma_prefix_weight prev 2}
+        weight_sum (slice w 0 c'') + weight (prefix prev 2);
+        <={}
+        weight_sum (slice w 0 c'') +
+        (max - e) * weight_sum (slice w 0 (prefix_coin_cnt prev 2));
+        <={
+          lemma_row_monotonous prev s';
+          lemma_weight_monotonous w (prefix_coin_cnt prev 2) c'';
+          Math.Lemmas.lemma_mult_le_left
+            (max - e)
+            (weight_sum (slice w 0 (prefix_coin_cnt prev 2)))
+            (weight_sum (slice w 0 c''))
+        }
+        weight_sum (slice w 0 c'') + (max - e) * weight_sum (slice w 0 c'');
+        <={Math.Lemmas.distributivity_add_left 1 (max - e) (weight_sum (slice w 0 c''))}
+        (max - e + 1) * weight_sum (slice w 0 c'');
+      }
+    else
+      let p'' = (p' + 1) * 2 in
+      calc (<=) {
+        weight (prefix s' i);
+        <={}
+        weight_sum (slice w 0 c'') + weight (prefix prev (p' * 2)) +
+        weight prev.(p' * 2) + weight prev.(p' * 2 + 1);
+        <={lemma_prefix_weight prev (p' * 2 + 1)}
+        weight_sum (slice w 0 c'') +
+        weight (prefix prev (p' * 2 + 1)) + weight prev.(p' * 2 + 1);
+        <={lemma_prefix_weight prev (p' * 2 + 2)}
+        weight_sum (slice w 0 c'') + weight (prefix prev p'');
+        <={}
+        weight_sum (slice w 0 c'') +
+        (max - e ) * weight_sum (slice w 0 (prefix_coin_cnt prev p''));
+        <={
+          lemma_row_monotonous prev s';
+          lemma_weight_monotonous w (prefix_coin_cnt prev p'') c'';
+          Math.Lemmas.lemma_mult_le_left
+            (max - e)
+            (weight_sum (slice w 0 (prefix_coin_cnt prev p'')))
+            (weight_sum (slice w 0 c''))
+        }
+        weight_sum (slice w 0 c'') + (max - e ) * weight_sum (slice w 0 c'');
+        <={Math.Lemmas.distributivity_add_left 1 (max - e) (weight_sum (slice w 0 c''))}
+        (max - e + 1) * weight_sum (slice w 0 c'');
+      }
+  end
+
+let lemma_pkg_weight_upper_bound_aux #w (#e: pos) (max: pos{max > e})
+  #p (prev: row w (e + 1) (length w) p{row_weight_upper_bound max prev})
+  #c' (#p': pkg_cnt c'{p' * 2 <= length w + p})
+  (s: row w e c' p'{row_weight_equality prev s /\ row_weight_upper_bound max s})
+  (i: pos{i <= c' + p' + 1}) : Lemma
+  (requires
+    merge_element_lt prev s /\
+    unpack_correspond prev s /\
+    (pkg_smaller prev s \/ coin_smaller prev s))
+  (ensures
+    (pkg_smaller prev s ==> (
+      let s' = SPackage s (Package prev.(p' * 2) prev.(p' * 2 + 1)) in
+      let c'' = prefix_coin_cnt s' i in
+      weight (prefix s' i) <= (max - e + 1) * weight_sum (slice w 0 c''))) /\
+    (coin_smaller prev s ==> (
+      let s' = SCoin s (Coin e w.[c']) in
+      let c'' = prefix_coin_cnt s' i in
+      weight (prefix s' i) <= (max - e + 1) * weight_sum (slice w 0 c'')))) =
+  let n = length w in
+  let pmax = Math.Lib.min (n - 2) ((n + p) / 2) in
+  if c' < n && (p' = pmax || weight prev.(p' * 2) + weight prev.(p' * 2 + 1) >= w.[c']) then
+    lemma_pkg_weight_upper_bound_coin_aux max prev s i
+  else
+    lemma_pkg_weight_upper_bound_pkg_aux max prev s i
+
+let lemma_pkg_weight_upper_bound #w (#e: pos) (max: pos{max > e})
+  #p (prev: row w (e + 1) (length w) p{row_weight_upper_bound max prev})
+  #c' (#p': pkg_cnt c'{p' * 2 <= length w + p})
+  (s: row w e c' p'{row_weight_equality prev s /\ row_weight_upper_bound max s}): Lemma
+  (requires
+    merge_element_lt prev s /\
+    unpack_correspond prev s /\
+    (pkg_smaller prev s \/ coin_smaller prev s))
+  (ensures
+    (pkg_smaller prev s ==>
+      row_weight_upper_bound max (SPackage s (Package prev.(p' * 2) prev.(p' * 2 + 1)))) /\
+    (coin_smaller prev s ==> row_weight_upper_bound max (SCoin s (Coin e w.[c'])))) =
+  forall_intro (move_requires (lemma_pkg_weight_upper_bound_aux max prev s))
+
+#push-options "--fuel 1 --ifuel 0"
+let lemma_pkg_weight #w #n #e #max #p prev #c' #p' s =
+  let pmax = Math.Lib.min (n - 2) ((n + p) / 2) in
   if 2 * p' + 3 < n + p then begin
     lemma_row_weight_sorted prev (p' * 2) (p' * 2 + 1);
     lemma_row_weight_sorted prev (p' * 2 + 1) (p' * 2 + 2);
     lemma_row_weight_sorted prev (p' * 2 + 2) (p' * 2 + 3)
   end;
+  if c' < n || p' < pmax then begin
+    lemma_pkg_weight_sorted prev s;
+    lemma_pkg_weight_unpack prev s;
+    lemma_pkg_weight_equality prev s;
+    lemma_pkg_weight_upper_bound max prev s;
+    lemma_pkg_weight_merge_inv max prev s
+  end;
 
-  let pmax = Math.Lib.min (n - 2) ((n + p) / 2) in
   match (c' < n, p' < pmax) with
-  | (false, true) -> lemma_last_item_gte_last_leaf s
+  | (false, true) -> lemma_last_item_gte_last_coin s
   | (true, true) -> 
-    let pkg: item (e - 1) _ = Package prev.(p' * 2) prev.(p' * 2 + 1) in
-    let coin = Coin (e - 1) w.[c'] in
-    if weight pkg < weight coin then lemma_last_item_gte_last_leaf s
+    let pkg: item e _ = Package prev.(p' * 2) prev.(p' * 2 + 1) in
+    let coin = Coin e w.[c'] in
+    if weight pkg < weight coin then lemma_last_item_gte_last_coin s
   | _ -> ()
 #pop-options
 
