specs/Spec.Package.Merge.fsti
@@ -16,7 +16,7 @@ class weight_value (a:Type) =
 type item: (exp: pos) -> (weight: pos) -> Type =
   | Coin: exp: pos -> weight: pos -> item exp weight
   | Package: #exp: pos -> #w1: pos -> #w2: pos ->
-      i1: item (exp + 1) w1 -> i2: item (exp + 1) w2 -> item exp (w1 + w2)
+    i1: item (exp + 1) w1 -> i2: item (exp + 1) w2 -> item exp (w1 + w2)
 
 instance item_weight_value #e #w: weight_value (item e w) =
 {
@@ -28,6 +28,11 @@ let rec weight_sorted (w: seq pos): Tot bool (decreases length w) =
   match length w with
   | 0 | 1 -> true
   | _ -> w.[0] <= w.[1] && weight_sorted (tail w)
+
+let rec weight_sum (w: seq pos{length w >= 1}): Tot pos (decreases length w) =
+  match length w with
+  | 1 -> last w
+  | _ -> weight_sum (unsnoc w) + last w
 
 type weights = w: seq pos{length w >= 2 /\ weight_sorted w}
 
@@ -68,7 +73,7 @@ let lt #e #w1 #w2 (i1: item e w1) (i2: item e w2) =
   | (false, true) -> w1 < w2
 
 private let rec row_item_weight #w #e #c #p
-  (s: row_t w e c p{c + p > 0}) (i: nat{i < c + p}): Tot pos =
+  (s: row_t w e c p) (i: nat{i < c + p}): Tot pos =
   match i = c + p - 1 with
   | true -> (match s with
     | SHead c -> weight (c <: item e w.[0])
@@ -76,32 +81,36 @@ private let rec row_item_weight #w #e #c #p
     | SPackage #_ #_ #_ #_ #wp xs x -> weight (x <: item e wp))
   | false -> (match s with | SCoin xs x | SPackage xs x -> row_item_weight xs i)
 
-private let rec row_index #w #e #c #p (s: row_t w e c p{c + p > 0}) (i: nat{i < c + p}):
+private let rec row_index #w #e #c #p (s: row_t w e c p) (i: nat{i < c + p}):
   Tot (item e (row_item_weight s i)) =
   match i = c + p - 1 with
   | true -> (match s with | SHead x -> x | SCoin xs x | SPackage xs x -> x)
   | false -> match s with | SCoin xs x | SPackage xs x -> row_index xs i
 
-let op_Array_Access #w #e #c #p (s: row_t w e c p{c + p > 0}) = row_index s
+let op_Array_Access #w #e #c #p (s: row_t w e c p) = row_index s
 
-type pkg_index #w (p: pkg_cnt #w (length w)) (c': coin_cnt w) = p': pkg_cnt c'{
-  p' <= length w - 2 /\ p' <= (length w + p) / 2
-}
+private let rec prefix_coin_cnt
+  #w #e #c #p (s: row_t w e c p) (i: pos{i <= c + p}): Tot (c': pos{c' <= c}) =
+  if i = c + p then
+    c
+  else
+    match s with | SCoin xs _ | SPackage xs _ -> prefix_coin_cnt xs i
 
-private unfold let prev_coin_cnt #w #e #c #p (s: row_t w e c p) =
-  match s with
-  | SCoin xs x -> c - 1
-  | _ -> c
+private let rec prefix_pkg_cnt #w #e #c #p (s: row_t w e c p) (i: pos{i <= c + p}):
+  Tot (pkg_cnt #w (prefix_coin_cnt s i)) =
+  if i = c + p then
+    p
+  else
+    match s with | SCoin xs _ | SPackage xs _ -> prefix_pkg_cnt xs i
 
-private unfold let prev_pkg_cnt #w #e #c #p (s: row_t w e c p) =
-  match s with
-  | SPackage xs x -> p - 1
-  | _ -> p
+let rec prefix #w #e #c #p (s: row_t w e c p) (i: pos{i <= c + p}):
+  Tot (row_t w e (prefix_coin_cnt s i) (prefix_pkg_cnt s i)) =
+  if i = c + p then
+    s
+  else
+    match s with | SCoin xs _ | SPackage xs _ -> prefix xs i
 
-let unsnoc #w #e #c #p (s: row_t w e c p{SHead? s == false}):
-  Tot (row_t w e (prev_coin_cnt s) (prev_pkg_cnt s)) =
-  match s with
-  | SCoin xs x | SPackage xs x -> xs
+unfold let unsnoc #w #e #c #p (s: row_t w e c p{SHead? s == false}) = prefix s (c + p - 1)
 
 let rec row_sorted #w #e #c #p (s: row_t w e c p): Tot bool =
   if c + p >= 2 then
@@ -131,22 +140,132 @@ private let rec unpack_correspond #w (#e: pos{e > 1}) #c #p #c' #p'
       prev.(j) = i1 && prev.(j + 1) = i2 &&
       unpack_correspond prev xs
 
+private let row_weight_upper_bound
+  #w (#e: pos) #c #p (max: pos{max >= e}) (s: row_t w e c p) =
+  forall i. weight (prefix s i) <= (max - e + 1) * weight_sum (slice w 0 (prefix_coin_cnt s i))
+
+private let row_weight_equality
+  (#w: weights) (#e: pos)
+  (#p: pkg_cnt #w (length w)) #c' (#p': pkg_cnt c'{p' * 2 <= length w + p})
+  (prev: row_t w (e + 1) (length w) p) (s: row_t w e c' p') =
+  (p' > 0 ==> weight s == weight_sum (slice w 0 c') + weight (prefix prev (p' * 2))) /\
+  (p' == 0 ==> weight s == weight_sum (slice w 0 c'))
+
+let merge_element_lt #w (#e: pos)
+  #p (prev: row_t w (e + 1) (length w) p{row_sorted prev})
+  #c' #p' (s: row_t w e c' p'{row_sorted s}) =
+  let n = length w in
+  let lst = s.(p' + c' - 1) in
+  (c' < n ==> lst `lt` Coin e w.[c']) /\
+  (2 * p' + 1 < n + p ==> lst `lt` Package prev.(2 * p') prev.(2 * p' + 1))
+
 #push-options "--fuel 0 --ifuel 0 --z3refresh"
-type row_partial #w (#e: pos) #p (prev: row w (e + 1) (length w) p) c' p' =
-  xs: row w e c' p' {
+type row_partial #w (#e: pos) #p (max: pos{max > e})
+  (prev: row w (e + 1) (length w) p) c' p' =
+  s: row w e c' p' {
     let n = length w in
     let lp = n + p in
-    unpack_correspond prev xs /\
-    (c' + p' > 0 ==>
-      (let lst = xs.(p' + c' - 1) in
-      (c' < n ==> lst `lt` Coin e w.[c']) /\
-      (2 * p' + 1 < lp ==> lst `lt` Package prev.(2 * p') prev.(2 * p' + 1))))
+    p' * 2 <= lp /\
+    unpack_correspond prev s /\
+    row_weight_upper_bound max s /\
+    row_weight_equality prev s /\
+    merge_element_lt prev s
   }
 #pop-options
+
+val lemma_weight_sorted: w: weights -> i: index_t w -> j: index_t w -> Lemma
+  (requires i <= j)
+  (ensures w.[i] <= w.[j])
+  (decreases %[length w; j - i])
+  [SMTPat w.[i]; SMTPat w.[j]]
+
+type pkg_index #w (p: pkg_cnt #w (length w)) (c': coin_cnt w) = p': pkg_cnt c'{
+  p' <= length w - 2 /\ p' <= (length w + p) / 2
+}
+
+#push-options "--z3rlimit 256 --fuel 1 --ifuel 1 --query_stats"
+let pkg_smaller
+  #w (#e: pos) #p (prev: row_t w (e + 1) (length w) p) #c' #p' (s: row_t w e c' p') =
+  let n = length w in
+  p' < Math.Lib.min (n - 2) ((n + p) / 2) /\
+  (c' < n ==> (
+    let pkg: item e _ = Package prev.(p' * 2) prev.(p' * 2 + 1) in
+    let coin = Coin e w.[c'] in
+    weight pkg < weight coin
+  ))
+
+let coin_smaller
+  #w (#e: pos) #p (prev: row_t w (e + 1) (length w) p) #c' #p' (s: row_t w e c' p') =
+  let n = length w in
+  c' < n /\
+  (p' < Math.Lib.min (n - 2) ((n + p) / 2) ==> (
+    let pkg: item e _ = Package prev.(p' * 2) prev.(p' * 2 + 1) in
+    let coin = Coin e w.[c'] in
+    weight coin <= weight pkg
+  ))
+
+private let table_row_pred (#w: weights) (#e: pos) (max: pos{max > e})
+  (#p: pkg_cnt (length w)) (prev: row w (e + 1) (length w) p)
+  #c' (#p': pkg_cnt c'{p' * 2 <= length w + p}) (s: row_t w e c' p') =
+  row_sorted s /\
+  row_pkg_gt s /\
+  row_weight_equality prev s /\
+  row_weight_upper_bound max s /\
+  unpack_correspond prev s /\
+  merge_element_lt prev s
+
+val lemma_pkg_weight:
+    #w: weights
+  -> #n: nat{n == length w}
+  -> #e: pos
+  -> #max: pos{max > e}
+  -> #p: pkg_cnt n{p <= n - 2}
+  -> prev: row w (e + 1) n p{row_weight_upper_bound max prev}
+  -> #c': pos{c' <= n}
+  -> #p': pkg_index p c'{p' <= 2 * length w + p}
+  -> s: row_partial #_ #e #_ max prev c' p'
+  -> Lemma
+  (requires c' < n \/ p' < Math.Lib.min (n - 2) ((n + p) / 2))
+  (ensures 
+    (2 * p' + 3 < n + p ==>
+      prev.(p' * 2) `lt` prev.(p' * 2 + 1) /\
+      prev.(p' * 2 + 1) `lt` prev.(p' * 2 + 2) /\
+      prev.(p' * 2 + 2) `lt` prev.(p' * 2 + 3)) /\
+    (pkg_smaller prev s ==> 
+      table_row_pred max prev (SPackage s (Package prev.(p' * 2) prev.(p' * 2 + 1)))) /\
+    (coin_smaller prev s ==> table_row_pred max prev (SCoin s (Coin e w.[c']))))
 
 unfold let next_pkg_cnt (w: weights) (p: nat): Tot nat =
   let n = length w in
   Math.Lib.min (n - 2) ((n + p) / 2) 
+
+#push-options "--fuel 1 --ifuel 0 --z3rlimit 1024 --z3refresh"
+let rec merge (#w: weights) (#n: nat{n == length w}) (#e: pos) (#max: pos{max >= e + 1})
+  (#p: pkg_cnt n{p <= n - 2}) (prev: row w (e + 1) n p{
+    row_weight_upper_bound max prev
+  }) (#c': pos{c' <= n}) (#p': pkg_index p c')
+  (s: row_partial max prev c' p'):
+  Tot (s': row w e n (next_pkg_cnt w p){
+    unpack_correspond prev s' /\
+    row_weight_upper_bound max s
+  }) (decreases %[n - c'; n + p - 2 * p']) =
+  let pmax = Math.Lib.min (n - 2) ((n + p) / 2) in
+  if c' < n || p' < pmax then lemma_pkg_weight prev s;
+
+  match (c' < n, p' < pmax) with
+  | (false, false) -> s
+  | (false, true) ->
+    merge #w #n #e #max #p prev (SPackage s (Package prev.(p' * 2) prev.(p' * 2 + 1)))
+  | (true, false) ->
+    merge #w #n #e #max #p prev (SCoin s (Coin e w.[c']))
+  | _ ->
+    let pkg: item e _ = Package prev.(p' * 2) prev.(p' * 2 + 1) in
+    let coin = Coin e w.[c'] in
+    if weight pkg < weight coin then 
+      merge #w #n #e #max #p prev (SPackage s pkg)
+    else
+      merge #w #n #e #max #p prev (SCoin s coin)
+#pop-options
 
 type table:
     w: weights
@@ -164,90 +283,3 @@ type table:
       s: row w (min - 1) (length w) (next_pkg_cnt w p){
         unpack_correspond prev s
       } -> table w max (min - 1) (next_pkg_cnt w p) s
-
-val lemma_weight_sorted: w: weights -> i: index_t w -> j: index_t w -> Lemma
-  (requires i <= j)
-  (ensures w.[i] <= w.[j])
-  (decreases %[length w; j - i])
-  [SMTPat w.[i]; SMTPat w.[j]]
-
-val lemma_row_weight_sorted:
-    #w: weights
-  -> #e: pos
-  -> #c: coin_cnt w
-  -> #p: pkg_cnt c
-  -> s: row_t w e c p{row_sorted s}
-  -> i: nat{i < c + p}
-  -> j: nat{j < c + p}
-  -> Lemma
-  (requires i < j)
-  (ensures s.(i) `lt` s.(j))
-  (decreases %[c + p; j - i])
-
-#push-options "--z3rlimit 256 --fuel 1 --ifuel 1 --query_stats"
-let pkg_smaller
-  (#w: weights) (#n: nat{n == length w}) (#e: pos{e > 1})
-  (#p: pkg_cnt n{p <= n - 2}) (#c': pos{c' <= n}) (#p': pkg_index p c')
-  (prev: row w e n p) (s: row_partial #_ #(e - 1) #_ prev c' p') =
-  p' < Math.Lib.min (n - 2) ((n + p) / 2) /\
-  (c' < n ==> (
-    let pkg: item (e - 1) _ = Package prev.(p' * 2) prev.(p' * 2 + 1) in
-    let coin = Coin (e - 1) w.[c'] in
-    weight pkg < weight coin
-  ))
-
-let coin_smaller
-  (#w: weights) (#n: nat{n == length w}) (#e: pos{e > 1})
-  (#p: pkg_cnt n{p <= n - 2}) (#c': pos{c' <= n}) (#p': pkg_index p c')
-  (prev: row w e n p) (s: row_partial #_ #(e - 1) #_ prev c' p') =
-  c' < n /\
-  (p' < Math.Lib.min (n - 2) ((n + p) / 2) ==> (
-    let pkg: item (e - 1) _ = Package prev.(p' * 2) prev.(p' * 2 + 1) in
-    let coin = Coin (e - 1) w.[c'] in
-    weight coin <= weight pkg
-  ))
-
-val lemma_pkg_weight:
-    #w: weights
-  -> #n: nat{n == length w}
-  -> #e: pos{e > 1}
-  -> #p: pkg_cnt n{p <= n - 2}
-  -> #c': pos{c' <= n}
-  -> #p': pkg_index p c'
-  -> prev: row w e n p
-  -> s: row_partial #_ #(e - 1) #_ prev c' p'
-  -> Lemma
-  (requires c' < n \/ p' < Math.Lib.min (n - 2) ((n + p) / 2))
-  (ensures 
-    (2 * p' + 3 < n + p ==>
-      prev.(p' * 2) `lt` prev.(p' * 2 + 1) /\
-      prev.(p' * 2 + 1) `lt` prev.(p' * 2 + 2) /\
-      prev.(p' * 2 + 2) `lt` prev.(p' * 2 + 3)) /\
-    (pkg_smaller prev s ==> 
-      row_pkg_gt (SPackage s (Package prev.(p' * 2) prev.(p' * 2 + 1)))
-    ) /\ (coin_smaller prev s ==> 
-      row_pkg_gt (SCoin s (Coin (e - 1) w.[c']))
-    ))
-
-#push-options "--fuel 1 --ifuel 0 --z3rlimit 1024"
-let rec merge (#w: weights) (#n: nat{n == length w}) (#e: pos{e > 1})
-  (#p: pkg_cnt n{p <= n - 2}) (#c': pos{c' <= n}) (#p': pkg_index p c')
-  (prev: row w e n p) (s: row_partial prev c' p'):
-  Tot (s': row w (e - 1) n (next_pkg_cnt w p){
-    unpack_correspond prev s'
-  }) (decreases %[n - c'; n + p - 2 * p']) =
-  let pmax = Math.Lib.min (n - 2) ((n + p) / 2) in
-  if c' < n || p' < pmax then lemma_pkg_weight prev s;
-
-  match (c' < n, p' < pmax) with
-  | (false, false) -> s
-  | (false, true) -> merge prev (SPackage s (Package prev.(p' * 2) prev.(p' * 2 + 1)))
-  | (true, false) -> merge prev (SCoin s (Coin (e - 1) w.[c']))
-  | _ ->
-    let pkg: item (e - 1) _ = Package prev.(p' * 2) prev.(p' * 2 + 1) in
-    let coin = Coin (e - 1) w.[c'] in
-    if weight pkg < weight coin then 
-      merge prev (SPackage s pkg)
-    else
-      merge prev (SCoin s coin)
-
